move MyBasicALU from BinarySearch.v to Basic_bopnames.v

bedrock2/src/Basic_bopnames.v
@@ -1,4 +1,23 @@
-Module bopname.
+Require bedrock2.Syntax.
+Require bedrock2.BasicALU.
+
+Module Import bopname.
   Inductive bopname := add | sub | mul | and | or | xor | sru | slu | srs | lts | ltu | eq.
 End bopname.
 Notation bopname := bopname.bopname.
+
+Class parameters := {
+  varname: Set;
+  funcname: Set;
+  actname: Set;
+}.
+
+Instance make (p: parameters) : Syntax.parameters := {|
+  Syntax.varname := @varname p;
+  Syntax.funname := @funcname p;
+  Syntax.actname := @actname p;
+  Syntax.bopname := bopname;
+|}.
+
+Instance BasicALU{p: parameters}: BasicALU.operations :=
+  BasicALU.Build_operations _ add sub mul and or xor sru slu srs lts ltu eq.
